QS.v
@@ -46,26 +46,26 @@ Proof.
 Qed.
 
 (* the number of items added by w^n is equal to the number of items added by w multiplied by n. *)
-Theorem count_word_pow: forall w n,
-  count_buffer (word_pow w n) = (Z.of_nat n) * (count_buffer w).
+Theorem count_str_pow: forall w n,
+  count_buffer (w^n) = (Z.of_nat n) * (count_buffer w).
 Proof.
   intros w n;
   induction n as [|n IH]; auto;
-  replace (word_pow w (S n)) with (w ++ word_pow w n); auto;
+  replace (w^(S n)) with (w ++ w^n); auto;
   rewrite count_buffer_distr, IH, Nat2Z.inj_succ, <- Zmult_succ_l_reverse;
   omega.
 Qed.
 
 (* a function that lists the sequences of events of a given list that transition into a given state *)
-Fixpoint gen_words q (l:list (list B)) :=
+Fixpoint gen_strings q (l:list (list B)) :=
   match l with
-  | w::l' => if A_eq_dec (ixtransition w) q then w::gen_words q l' else gen_words q l'
+  | w::l' => if A_eq_dec (ixtransition w) q then w::gen_strings q l' else gen_strings q l'
   | nil => nil
   end.
 
-(* Every sequence of events returned by gen_words must be correct. *)
-Lemma gen_words_correct q l : forall w,
-  In w (gen_words q l) -> ixtransition w = q.
+(* Every sequence of events returned by gen_strings must be correct. *)
+Lemma gen_strings_correct q l : forall w,
+  In w (gen_strings q l) -> ixtransition w = q.
 Proof.
   intros w H0;
   induction l as [|w' l' IH].
@@ -82,9 +82,9 @@ Proof.
       1,2: apply IH; auto.
 Qed.
 
-(* Every sequence of events in l that transitions into q is in gen_words q l. *)
-Lemma gen_words_complete q l : forall w,
-  In w l -> ixtransition w = q -> In w (gen_words q l).
+(* Every sequence of events in l that transitions into q is in gen_strings q l. *)
+Lemma gen_strings_complete q l : forall w,
+  In w l -> ixtransition w = q -> In w (gen_strings q l).
 Proof.
   intros w H H0.
   induction l as [|w' l' IH]; inversion H; simpl.
@@ -97,17 +97,17 @@ Qed.
 
 (* a function that lists the sequences of events of a given list that transition into a given state
   and whose length is less or equal to a given number *)
-Definition all_gen_words_le q n := gen_words q (all_words_le n).
+Definition all_gen_strings_le q n := gen_strings q (all_words_le n).
 
 (* Every generated sequence of events that transition into q and whose length is less or equal to n
-  is in all_gen_words_le q n. *)
-Lemma all_gen_words_le_generated q n : forall w,
+  is in all_gen_strings_le q n. *)
+Lemma all_gen_strings_le_generated q n : forall w,
   q <> sink -> ixtransition w = q -> (length w <= n)%nat ->
-  In w (all_gen_words_le q n).
+  In w (all_gen_strings_le q n).
 Proof.
-  unfold all_gen_words_le;
+  unfold all_gen_strings_le;
   intros w H H0 H1;
-  apply gen_words_complete.
+  apply gen_strings_complete.
   apply all_words_le_generated;
   rewrite <- H0 in H.
   1-3: auto.
