QSUpperBound.v
@@ -83,16 +83,16 @@ Proof.
       omega.
     + rewrite H2, count_buffer_distr, count_buffer_distr, count_buffer_distr;
       omega.
-  - assert (contra: init_items + count_buffer (w1 ++ word_pow w2 (S m) ++ w3) > max_items). {
+  - assert (contra: init_items + count_buffer (w1 ++ w2^(S m) ++ w3) > max_items). {
       rewrite count_buffer_distr, count_buffer_distr;
-      rewrite count_word_pow.
+      rewrite count_str_pow.
       replace (count_buffer w1 + (Z.of_nat (S m) * count_buffer w2 + count_buffer w3)) with
       (count_buffer w + Z.of_nat m * count_buffer w2).
       2: rewrite H2; rewrite count_buffer_distr, count_buffer_distr;
       rewrite Nat2Z.inj_succ, <- Z.add_1_r, Z.mul_add_distr_r; omega.
       nia.
     }
-    assert (contra0: generates (w1 ++ word_pow w2 (S m) ++ w3)).
+    assert (contra0: generates (w1 ++ w2^(S m) ++ w3)).
       unfold generates; fold ixtransition; rewrite H4, H0;
       auto.
     apply H in contra0. omega.
@@ -151,8 +151,8 @@ Proof.
       -- rewrite app_length in H3; simpl in H3; omega.
 Qed.
 
-(* max_word q w is True if w counts the minimum items in q (maximum word) *)
-Definition max_word q w :=
+(* max_string q w is True if w counts the minimum items in q (maximum string) *)
+Definition max_string q w :=
   ixtransition w = q /\ forall w', ixtransition w' = q -> count_buffer w' <= count_buffer w.
 
 (* a function that takes w1 and w2 and returns the sequence that counts most items *)
@@ -244,42 +244,42 @@ Qed.
 
 (* a function that returns the generated sequence of events w of length less than the number of states
   such that w transitions into q and adds most items *)
-Definition max_gen_words q := max_list (all_gen_words_le q (length states - 1)).
+Definition max_gen_strings q := max_list (all_gen_strings_le q (length states - 1)).
 
-(* If the queueing system is upper bounded, every tangible state q is upper bounded. max_gen_words q must
+(* If the queueing system is upper bounded, every tangible state q is upper bounded. max_gen_strings q must
   count the maximum items in q. *)
-Lemma max_gen_words_correct q :
+Lemma max_gen_strings_correct q :
   upper_bounded -> is_tangible q ->
-  max_word q (max_gen_words q).
+  max_string q (max_gen_strings q).
 Proof.
   intros H H0.
-  unfold max_word.
-  split; unfold max_gen_words.
+  unfold max_string.
+  split; unfold max_gen_strings.
   - apply max_list_state.
     + apply tangible_length in H0; destruct H0 as [w [H0 [H1 H2]]]; fold ixtransition in H0.
-      eapply all_gen_words_le_generated with (n:=(length states - 1)%nat) in H2.
+      eapply all_gen_strings_le_generated with (n:=(length states - 1)%nat) in H2.
       2: apply H0.
       2: omega.
       intro contra; rewrite contra in H2; destruct H2.
-    + intros w H1; unfold all_gen_words_le in H1;
-      eapply gen_words_correct. apply H1.
+    + intros w H1; unfold all_gen_strings_le in H1;
+      eapply gen_strings_correct. apply H1.
   - intros w H1;
     destruct H0 as [H0 H2];
     destruct (le_gt_dec (length w) (length states - 1)).
-    + apply max_list_correct, all_gen_words_le_generated; auto.
+    + apply max_list_correct, all_gen_strings_le_generated; auto.
     + assert (H3: (length w >= length states)%nat). omega.
       eapply pumping_buffer with (q:=q) in H3.
       2-4: auto.
       destruct H3 as [w' [H3 [H4 H5]]].
-      assert (count_buffer w' <= count_buffer (max_list (all_gen_words_le q (length states - 1)))).
-        apply max_list_correct, all_gen_words_le_generated; auto; omega.
+      assert (count_buffer w' <= count_buffer (max_list (all_gen_strings_le q (length states - 1)))).
+        apply max_list_correct, all_gen_strings_le_generated; auto; omega.
       omega.
 Qed.
 
-(* The initial state's maximum word does not add items to the buffer if the queueing system is bounded. *)
-Lemma max_word_state0 : forall w,
+(* The initial state's maximum string does not add items to the buffer if the queueing system is bounded. *)
+Lemma max_string_state0 : forall w,
   upper_bounded ->
-  max_word state0 w ->
+  max_string state0 w ->
   count_buffer w = 0.
 Proof.
   intros w H H0.
@@ -288,7 +288,7 @@ Proof.
   - auto.
   - pose proof (Zgt_pos_0 p) as H2; rewrite <- H1 in H2, H3;
     clear H1; pose H0 as H1; apply state0_cycle with (n:=2%nat) in H1;
-    apply H3 in H1. unfold count_buffer in H1; rewrite count_word_pow in H1; fold count_buffer in H1.
+    apply H3 in H1. unfold count_buffer in H1; rewrite count_str_pow in H1; fold count_buffer in H1.
     nia.
   - pose proof (Zlt_neg_0 p) as H2; rewrite <- H1 in H2;
     clear H0; assert (H0: ixtransition [] = state0). auto.
@@ -297,9 +297,9 @@ Proof.
 Qed.
 
 (* a lemma related to the second constraint of the function f *)
-Lemma max_word_transition : forall q e qe w we,
+Lemma max_string_transition : forall q e qe w we,
   transition q e = qe -> qe <> sink ->
-  max_word q w -> max_word qe we ->
+  max_string q w -> max_string qe we ->
   count_buffer we >= count_buffer w + count_event e.
 Proof.
   intros q e qe w we H H0 H1 H2.
@@ -330,18 +330,18 @@ Proof.
     apply buffer_count_leq_f; try split; try (apply H0); intuition.
 
   - intro H.
-    exists (fun q => if A_eq_dec q sink then (max_items)+(max_count_event) else (init_items) + count_buffer (max_gen_words q)).
+    exists (fun q => if A_eq_dec q sink then (max_items)+(max_count_event) else (init_items) + count_buffer (max_gen_strings q)).
     split.
     + destruct (A_eq_dec state0 sink) as [H2|H2].
       destruct sink_correct as [_ [contra _]]; symmetry in H2; contradiction.
       assert (H1: is_tangible state0). split. auto. exists []; auto.
-      apply max_word_state0 with (w:=max_gen_words state0) in H.
+      apply max_string_state0 with (w:=max_gen_strings state0) in H.
       omega.
-      apply max_gen_words_correct; auto.
+      apply max_gen_strings_correct; auto.
     + intros q H0 H4; pose H4 as H1; destruct H1 as [H1 [w H2]].
       destruct (A_eq_dec q sink) as [H3|_]. contradiction.
-      assert (H5: generates (max_gen_words q)). {
-          apply (max_gen_words_correct q) in H. 2: auto.
+      assert (H5: generates (max_gen_strings q)). {
+          apply (max_gen_strings_correct q) in H. 2: auto.
           destruct H as [H _]; unfold generates; rewrite H; auto.
       }
       split.
@@ -349,11 +349,11 @@ Proof.
       * intros e H3;
         destruct (A_eq_dec (transition q e) sink).
         apply max_count_event_correct in H3.
-        assert (init_items + count_buffer (max_gen_words q) <= max_items). auto.
+        assert (init_items + count_buffer (max_gen_strings q) <= max_items). auto.
         omega.
-        assert (count_buffer (max_gen_words (transition q e)) >= count_buffer (max_gen_words q) + count_event e). {
-          apply max_word_transition with (q:=q)(qe:=transition q e); auto.
-          1,2: apply max_gen_words_correct; auto.
+        assert (count_buffer (max_gen_strings (transition q e)) >= count_buffer (max_gen_strings q) + count_event e). {
+          apply max_string_transition with (q:=q)(qe:=transition q e); auto.
+          1,2: apply max_gen_strings_correct; auto.
           split. auto.
           exists (w ++ [e]); rewrite ixtransition_distr, H2; auto.
         }
